operations/Linearize_rail.thy
@@ -1,17 +1,13 @@
 theory Linearize_rail
-  imports "Binders.MRBNF_Composition" "Binders.MRBNF_Recursor"
-  keywords "linearize_mrbnf" :: thy_goal
+  imports "Binders.MRBNF_Composition"
 begin
-
-ML_file "../Tools/mrbnf_linearize_tactics.ML"
-ML_file "../Tools/mrbnf_linearize.ML"
 (* this is just to build the rail diagram for linearize_mrbnf*)
 
 ML_file \<open>~~/src/Doc/antiquote_setup.ML\<close>
 text  \<open>
 \<^rail>\<open>
-  @@{command linearize_mrbnf} @{syntax spec} name '=' term @{syntax wits}? \<newline>
-    @'on' (typefree + @'and') @{syntax bindings}? (@'morphisms' name name)?
+  @@{command linearize_mrbnf} @{syntax spec} name '=' typ @{syntax wits}? \<newline>
+    @'on' (typefree + @'and') @{syntax bindings}? @{syntax 'morphisms'}?
   ;
   @{syntax_def spec}: @{syntax tfree} | '(' (((name ':')? @{syntax tfree}) + ',') ')'
   ;
@@ -20,21 +16,8 @@ text  \<open>
   @{syntax_def wits}: '[' 'wits' ':' (term + ',') ']'
   ;
   @{syntax_def bindings}: @'for' ((('map' | 'rel' | 'pred' | 'nonrep' | 'sameShape') ':' name) +)
-\<close>
-\<close>
-
-text  \<open>
-\<^rail>\<open>
-  @@{command linearize_mrbnf} @{syntax spec} name '=' term @{syntax wits}? \<newline>
-    @'on' (typefree + @'and') @{syntax bindings}
   ;
-  @{syntax_def spec}: @{syntax tfree} | '(' (((name ':')? @{syntax tfree}) + ',') ')'
-  ;
-  @{syntax_def tfree}: typefree ('::' sort)
-  ;
-  @{syntax_def wits}: '[' 'wits' ':' (term + ',') ']'
-  ;
-  @{syntax_def bindings}: (@'for' ((('map' | 'rel' | 'pred' | 'nonrep' | 'sameShape') ':' name) +))? (@'morphisms' name name)?
+  @{syntax_def 'morphisms'}: @'morphisms' name name
 \<close>
 \<close>
 end
